Preliminary runs for fuzzing + STLC

examples/fuzz-stlc/lambda.v
@@ -7,12 +7,33 @@ Import QcNotation.
 Import MonadNotation.
 Import ListNotations.
 
-Inductive type : Type :=
-| Base  : type
-| Fun   : type -> type -> type.
+(** Types *)
+
+Inductive Typ :=
+| Base  : Typ
+| Fun   : Typ -> Typ -> Typ.
 
 Notation "%" := Base.
 Notation "x :-> y" := (Fun x y) (at level 50).
+
+Derive (Arbitrary, Fuzzy) for Typ.
+
+Instance dec_eq_Typ (τ1 τ2 : Typ) : Dec (τ1 = τ2).
+Proof. dec_eq. Defined.
+
+(** Terms *)
+
+Inductive Term :=
+| Unit  : Term
+| Var   : nat -> Term
+| Lam   : Typ -> Term -> Term
+| App   : Term -> Term -> Term.
+
+Notation "#" := Unit.
+
+Derive (Arbitrary, Fuzzy) for Term.
+
+(** Printing *)
 
 Inductive Prec := POuter | PApp | PInner.
 
@@ -26,31 +47,16 @@ Definition ltp (p1 p2 : Prec) :=
 
 Definition parens outer inner s := if ltp inner outer then "(" ++ s ++ ")" else s.
 
-Fixpoint showType' prec (τ : type) :=
+Fixpoint showTyp' prec (τ : Typ) :=
   match τ with
   | Base => "()"
-  | Fun τ1 τ2 => parens prec PApp (showType' PInner τ1 ++ "->" ++ showType' PApp τ2)
+  | Fun τ1 τ2 => parens prec PApp (showTyp' PInner τ1 ++ "->" ++ showTyp' PApp τ2)
   end.
 
-Instance show_type : Show type :=
-  { show := showType' POuter }.
+Instance show_Typ : Show Typ :=
+  { show := showTyp' POuter }.
 
-Derive (Arbitrary, Fuzzy) for type.
-
-Instance dec_eq_type (τ1 τ2 : type) : Dec (τ1 = τ2).
-Proof. dec_eq. Defined.
-
-Inductive term : Type :=
-| Unit  : term
-| Var   : nat -> term
-| Lam   : type -> term -> term
-| App   : term -> term -> term.
-
-Notation "#" := Unit.
-
-Derive (Arbitrary, Fuzzy) for term.
-
-Fixpoint showExpr' prec (e : term) :=
+Fixpoint showExpr' prec (e : Term) :=
   match e with
   | Unit => "#"
   | Var x => show x
@@ -58,12 +64,47 @@ Fixpoint showExpr' prec (e : term) :=
   | App e1 e2 => parens prec PApp (showExpr' PApp e1 ++ " " ++ showExpr' PInner e2)
   end.
 
-Instance show_term : Show term :=
+Instance show_Term : Show Term :=
   { show := showExpr' POuter }.
 
-Definition env := list type.
+(** Mutants *)
 
-Inductive typing (Γ : env) : term -> type -> Prop :=
+Inductive Mutant :=
+| NoMutant
+| SubstNoLift
+| SubstNoIncr
+| SubstNoDecr
+| LiftAllVar
+| LiftLamNoIncr
+| LiftLamNoLift.
+
+Definition all_mutants :=
+  [ NoMutant
+  ; SubstNoLift
+  ; SubstNoIncr
+  ; SubstNoDecr
+  ; LiftAllVar
+  ; LiftLamNoIncr
+  ; LiftLamNoLift
+  ].
+
+Derive Show for Mutant.
+
+Instance dec_eq_Mutant (m1 m2 : Mutant) : Dec (m1 = m2).
+Proof. dec_eq. Defined.
+
+Fixpoint mut {A} (c : Mutant) (x : A)
+                 (my : list (Mutant * A)) : A :=
+  match my with
+  | [] => x
+  | (m,y) :: my' => if c = m? then y else mut c x my'
+  end.
+
+(** Typing *)
+
+Definition env := list Typ.
+
+Inductive typing (Γ : env) : Term -> Typ -> Prop :=
 | TBase : typing Γ Unit Base
 | TVar  : forall x τ, nth_error Γ x = Some τ -> typing Γ (Var x) τ
 | TLam  : forall e τ1 τ2, typing (τ1 :: Γ) e τ2 -> typing Γ (Lam τ1 e) (τ1 :-> τ2)
@@ -71,7 +112,7 @@ Inductive typing (Γ : env) : term -> type -> Prop :=
                               typing Γ e2 τ1 ->
                               typing Γ (App e1 e2) τ2.
 
-Fixpoint typeOf (Γ : env) (e : term) : option type :=
+Fixpoint typeOf (Γ : env) (e : Term) : option Typ :=
   match e with
   | Unit => Some Base
   | Var x => nth_error Γ x
@@ -87,59 +128,65 @@ Fixpoint typeOf (Γ : env) (e : term) : option type :=
                  end
   end.
 
-Definition well_typed (e : term) : bool :=
+Definition well_typed (e : Term) : bool :=
   match typeOf [] e with
   | Some _ => true
   | _ => false
   end.
 
-Fixpoint lift (n : nat) (e : term) : term :=
+Fixpoint lift (c : Mutant) (n : nat) (e : Term) : Term :=
   match e with
   | Unit      => Unit
-  | Var x     => Var (if x <? n then x else x+1)
-  | Lam τ e'  => Lam τ (lift (n+1) e')
-  | App e1 e2 => App (lift n e1) (lift n e2)
+  | Var x     => mut c (Var (if x <? n then x else x+1))
+                       [(LiftAllVar, Var (x+1))]
+  | Lam τ e'  => mut c (Lam τ (lift c (n+1) e'))
+                       [ (LiftLamNoIncr, Lam τ (lift c n e'))
+                       ; (LiftLamNoLift, Lam τ e') ]
+  | App e1 e2 => App (lift c n e1) (lift c n e2)
   end.
 
-Fixpoint subst (n : nat) (s : term) (e : term) : term :=
+Fixpoint subst (c : Mutant) (n : nat) (s : Term) (e : Term) : Term :=
   match e with
   | Unit  => Unit
   | Var x =>
     if x =? n then s
-    else if x <? n then Var (x-1)
+    else if n <? x then mut c (Var (x-1))
+                              [ (SubstNoDecr, Var x) ]
     else Var x
-  | Lam τ e' => Lam τ (subst (n+1) (lift 0 s) e')
-  | App e1 e2 => App (subst n s e1) (subst n s e2)
+  | Lam τ e' => mut c (Lam τ (subst c (n+1) (lift c 0 s) e'))
+                      [ (SubstNoIncr, Lam τ (subst c n (lift c 0 s) e'))
+                      ; (SubstNoLift, Lam τ (subst c (n+1) s e')) ]
+  | App e1 e2 => App (subst c n s e1) (subst c n s e2)
   end.
 
 (* Parallel reduction *)
-Fixpoint pstep (e : term) : term :=
+Fixpoint pstep (c : Mutant) (e : Term) : Term :=
   match e with
   | Unit  => Unit
   | Var x => Var x
-  | Lam τ e'  => Lam τ (pstep e')
-  | App e1 e2 => let e1' := pstep e1 in
-                 let e2' := pstep e2 in
+  | Lam τ e'  => Lam τ (pstep c e')
+  | App e1 e2 => let e1' := pstep c e1 in
+                 let e2' := pstep c e2 in
                  match e1' with
-                 | Lam τ body => subst 0 e2' body
+                 | Lam τ body => subst c 0 e2' body
                  | _ => App e1' e2'
                  end
   end.
 
 (* Generation *)
 
-Fixpoint gen_type (n : nat) : G type :=
+Fixpoint gen_Typ (n : nat) : G Typ :=
   match n with
   | O => ret Base
   | S n' => oneOf  [ ret Base
-                   ; τ1 <- gen_type (n' - 1);;
-                     τ2 <- gen_type n';;
+                   ; τ1 <- gen_Typ (n' - 1);;
+                     τ2 <- gen_Typ n';;
                      ret (τ1 :-> τ2)
                    ]
   end.
 
-Fixpoint gen_small_expr (Γ : env) (τ : type) : G term :=
-  let vars : list term :=
+Fixpoint gen_small_expr (Γ : env) (τ : Typ) : G Term :=
+  let vars : list Term :=
       map (fun '(n, τ') => Var n)
           (filter (fun '(n, τ') => τ = τ'?)
                   (combine (seq 0 (List.length Γ)) Γ)) in
@@ -150,7 +197,7 @@ Fixpoint gen_small_expr (Γ : env) (τ : type) : G term :=
               end  in
   oneOf_ base (base :: map ret vars).
 
-Fixpoint gen_expr (n : nat) (Γ : env) (τ : type) : G term :=
+Fixpoint gen_expr (n : nat) (Γ : env) (τ : Typ) : G Term :=
   match n with
   | O    => gen_small_expr Γ τ
   | S n' =>
@@ -161,36 +208,52 @@ Fixpoint gen_expr (n : nat) (Γ : env) (τ : type) : G term :=
                 | _ => []
                 end in
     let gApp :=
-        τ1 <- gen_type (min n 5);;
+        τ1 <- gen_Typ (min n 5);;
         e1 <- gen_expr n' Γ (τ1 :-> τ);;
         e2 <- gen_expr n' Γ τ1;;
         ret (App e1 e2) in
     oneOf_ (gen_small_expr Γ τ)
            ([ gen_small_expr Γ τ] ++ gLam ++ [gApp])
   end.
-           
+
+Fixpoint shrink_expr (τ : Typ) (t : Term) : list Term :=
+  List.filter (fun t' => typeOf [] t' = Some τ?) (shrink t ++ List.concat (List.map shrink (shrink t))).
+
 (* Sample (gen_expr 3 [] (Base :-> Base)). *)
 Definition prop_gen_wt :=
-  forAll (gen_type 5) (fun τ =>
+  forAll (gen_Typ 5) (fun τ =>
   forAll (gen_expr 6 [] τ) (fun e =>
   typeOf [] e = Some τ?)). 
 
-QuickChick prop_gen_wt.
+(* QuickChick prop_gen_wt. *)
 
-Definition preservation (e : term) :=
+Definition preservation (c : Mutant) (e : Term) :=
   match typeOf [] e with
   | Some τ =>
     whenFail ("Expr: " ++ show e ++ nl ++
-              "With type: " ++ show (typeOf [] e) ++ nl ++
-              "Steps to: " ++ show (pstep e) ++ nl ++
-              "With type: " ++ show (typeOf [] (pstep e)))
-             (typeOf [] (pstep e) = Some τ?)
+              "With Typ: " ++ show (typeOf [] e) ++ nl ++
+              "Steps to: " ++ show (pstep c e) ++ nl ++
+              "With Typ: " ++ show (typeOf [] (pstep c e)))
+             (typeOf [] (pstep c e) = Some τ?)
   | _ => checker tt
   end.
 
-Definition prop_preservation :=
-  forAll (gen_type 1) (fun τ =>
-  forAll (gen_expr 2 [] τ) (fun e =>
-  preservation e)).
+Definition preservation' (c : Mutant) (e : Term) : option bool := 
+  match typeOf [] e with
+  | Some τ =>
+    Some (typeOf [] (pstep c e) = Some τ?)
+  | _ => None
+  end.
 
-QuickCheck prop_preservation.
+Definition prop_preservation_smart (c : Mutant) :=
+  forAll (gen_Typ 3) (fun τ =>
+  forAllShrink (gen_expr 6 [] τ) (shrink_expr τ) (fun e =>
+  preservation c e)).
+
+Definition prop_preservation_naive (c : Mutant) := 
+  forAll arbitrary (preservation c).
+
+ManualExtract [Term; Typ; Mutant].
+Extract Constant defNumTests => "200000".
+
+(* QuickChick (prop_preservation NoMutant). *)
