examples/fuzz-stlc/fuzz_driver.sh
@@ -1,0 +1,16 @@
+#!/bin/bash
+
+for i in `seq $1 $2`; do
+    echo "Handling mutant #: $i"
+    cp lambda.v Tmp.v
+    echo "Definition prop_specialized (e : Term) : option bool :=" >> Tmp.v
+    echo "  let c := List.nth $i all_mutants NoMutant in" >> Tmp.v
+    echo "  preservation' c e." >> Tmp.v
+    echo "" >> Tmp.v
+    echo "Definition fuzzLoop :=" >> Tmp.v
+    echo "  fun _ : unit =>" >> Tmp.v
+    echo "    fuzzLoop arbitrary fuzz show prop_specialized." >> Tmp.v
+    echo "" >> Tmp.v
+    echo "FuzzQC SSNI_p (fuzzLoop tt). " >> Tmp.v
+    coqc Tmp.v -Q . QuickChick.FuzzSTLC &> output/qc_fuzz_${i}.out
+done
