examples/fuzz-stlc/rand_driver.sh
@@ -1,0 +1,12 @@
+#!/bin/bash
+
+for i in `seq $1 $2`; do
+    echo "Handling mutant #$i with generator $3"
+    cp lambda.v Tmp.v
+    echo "Definition prop_specialized :=" >> Tmp.v
+    echo "  let c := List.nth $i all_mutants NoMutant in" >> Tmp.v
+    echo "  prop_preservation_$3 c." >> Tmp.v
+    echo "" >> Tmp.v
+    echo "QuickChick prop_specialized. " >> Tmp.v
+    coqc Tmp.v -Q . QuickChick.FuzzSTLC &> output/qc_$3_${i}.out
+done
